lava/out/Benchmark/SafeIndexing.v
@@ -691,27 +691,27 @@ Proof.
                  ∧ ∃ (append_res : IList_u),
                    append_rel (Cons_u y ys) ds_d4Wt append_res
                    ∧ ∃ (get_res_2 : Z), get_rel append_res addZ_res get_res_2 ∧ get_res == get_res_2)
-            (let _: ∃ (get_res : Z),
-                    get_rel
-                    ⌊ append
-                      (exist (λ (l : IList_u), IList_wf l ∧ True) ys ltac:(solver))
-                      (exist (λ (ds_d4Wt : IList_u), IList_wf ds_d4Wt ∧ True) ds_d4Wt ltac:(solver)) -⌋
-                    (ds_d4Wv + ⌊ llen (exist (λ (l : IList_u), IList_wf l ∧ True) ys ltac:(solver)) -⌋)
-                    get_res
-                    ∧ ∃ (addZ_res : Z),
-                      addZ_rel
-                      (ds_d4Wv + ⌊ llen (exist (λ (l : IList_u), IList_wf l ∧ True) ys ltac:(solver)) -⌋)
-                      1
-                      addZ_res
-                      ∧ ∃ (get_res_2 : Z),
-                        get_rel
-                        (Cons_u y
-                         ⌊ append
-                           (exist (λ (l : IList_u), IList_wf l ∧ True) ys ltac:(solver))
-                           (exist (λ (ds_d4Wt : IList_u), IList_wf ds_d4Wt ∧ True) ds_d4Wt ltac:(solver)) -⌋)
-                        addZ_res
-                        get_res_2
-                        ∧ get_res == get_res_2 :=
+            (let H_38716321: ∃ (get_res : Z),
+                             get_rel
+                             ⌊ append
+                               (exist (λ (l : IList_u), IList_wf l ∧ True) ys ltac:(solver))
+                               (exist (λ (ds_d4Wt : IList_u), IList_wf ds_d4Wt ∧ True) ds_d4Wt ltac:(solver)) -⌋
+                             (ds_d4Wv + ⌊ llen (exist (λ (l : IList_u), IList_wf l ∧ True) ys ltac:(solver)) -⌋)
+                             get_res
+                             ∧ ∃ (addZ_res : Z),
+                               addZ_rel
+                               (ds_d4Wv + ⌊ llen (exist (λ (l : IList_u), IList_wf l ∧ True) ys ltac:(solver)) -⌋)
+                               1
+                               addZ_res
+                               ∧ ∃ (get_res_2 : Z),
+                                 get_rel
+                                 (Cons_u y
+                                  ⌊ append
+                                    (exist (λ (l : IList_u), IList_wf l ∧ True) ys ltac:(solver))
+                                    (exist (λ (ds_d4Wt : IList_u), IList_wf ds_d4Wt ∧ True) ds_d4Wt ltac:(solver)) -⌋)
+                                 addZ_res
+                                 get_res_2
+                                 ∧ get_res == get_res_2 :=
              ⌈ thm1
                (subsumptionCast
                 IList_u
